theories/examples/fibonacci__opaque.v
@@ -1,4 +1,0 @@
-From examples Require Import
-  fibonacci__code.
-
-#[global] Opaque fibonacci_fibonacci.
