theories/examples/future_fibonacci__opaque.v
@@ -1,0 +1,4 @@
+From examples Require Import
+  future_fibonacci__code.
+
+#[global] Opaque future_fibonacci_fibonacci.
